partial functions in models
to improve composability of models

also, rework of frontend

languages/fail-invalid-semantics/run.ml
@@ -1,14 +1,15 @@
+open Core
+open Printf
+open Libminuskapluginbase
+open Pluginbase
 
-      open Core
-      open Printf
-
-      let main () =
-        Libminuska.Miskeleton.main
-          Internal.chosen_builtins
-          (fun _ -> failwith "Parser not implemented.")
-          Internal.lang_interpreter
-          Internal.lang_interpreter_ext
-          Internal.lang_debug_info
-        
-      let _ = main ()
+let main () =
+  Libminuska.Miskeleton.main
+    (get_primitive_value_algebra (coqModuleName_of_sexp (Sexp.of_string ("(Std_module klike)"))))
+    (get_pi (coqModuleName_of_sexp (Sexp.of_string ("(Std_module trivial)"))))
+    Transform.parse
+    Internal.langDefaults
+    Internal.lang_Decls
+  
+let _ = main ()
     
