languages/fail-invalid-semantics/transform.ml
@@ -1,0 +1,8 @@
+open Core
+
+let convert_int (n : int) : Libminuska.Syntax.groundterm =
+  `GTb ({br_kind="int"; br_value=(sprintf "%d" n)})
+      
+let parse (lexbuf : Lexing.lexbuf) : Libminuska.Syntax.groundterm =
+  convert_int 42
+    
