languages/two-counters/run.ml
@@ -1,9 +1,15 @@
+open Base
+open Core
+open Libminuskapluginbase
+open Pluginbase
+open Syntax
+
 let main () =
   Libminuska.Miskeleton.main
-    Internal.chosen_builtins
+    (get_primitive_value_algebra (coqModuleName_of_sexp (Sexp.of_string ("(Std_module klike)"))))
+    (get_pi (coqModuleName_of_sexp (Sexp.of_string ("(Std_module trivial)"))))
     Transform.parse
-    Internal.lang_interpreter
-    Internal.lang_interpreter_ext
-    Internal.lang_debug_info
+    Internal.langDefaults
+    Internal.lang_Decls
   
 let _ = main ()
