minuska/lib/lexer.mll
@@ -16,12 +16,12 @@ let newline = '\r' | '\n' | "\r\n"
 let id = ['a'-'z'] ['a'-'z' 'A'-'Z' '0'-'9' '_' '.']*
 let var = ['A'-'Z' '_'] ['a'-'z' 'A'-'Z' '0'-'9' '_']*
 
-
 rule read =
   parse
   | white        { read lexbuf }
   | newline  { Lexing.new_line lexbuf; read lexbuf }
   | int      { INT (int_of_string (Lexing.lexeme lexbuf)) }
+  | '"'      { read_string (Buffer.create 17) lexbuf }
   | '('          { BRACKET_ROUND_LEFT }
   | ')'          { BRACKET_ROUND_RIGHT }
   | '['          { BRACKET_SQUARE_LEFT }
@@ -31,8 +31,8 @@ rule read =
   | "@frames"       { KEYWORD_FRAMES }
   | "@rule"       { KEYWORD_RULE }
   | "@context"       { KEYWORD_CONTEXT }
-  | "@builtin-int"       { KEYWORD_BUILTIN_INT }
-  | "@builtin-string"       { KEYWORD_BUILTIN_STRING }
+  | "@builtin"       { KEYWORD_BUILTIN }
+  | "@query"       { KEYWORD_QUERY }
   | "@true"       { KEYWORD_TRUE }
   | "@false"       { KEYWORD_FALSE }
   | "@and"       { KEYWORD_AND }
@@ -42,15 +42,30 @@ rule read =
   | "where"      { KEYWORD_WHERE }
   | "/"          { SLASH }
   | "=>"         { ARROW }
-  | "\""         { QUOTE }
+  (* | "\""         { QUOTE } *)
   | ";"          { SEMICOLON }
   | ":"          { COLON }
   | ':'          { COLON }
   | ','          { COMMA }
-
-  | int          { INT (int_of_string (Lexing.lexeme lexbuf)) }
   | id           { ID (Lexing.lexeme lexbuf)  }
   | var           { VAR (Lexing.lexeme lexbuf)  }
 
   | _            { raise (SyntaxError ("Unexpected char: " ^ Lexing.lexeme lexbuf)) }
   | eof          { EOF }
+(* from https://dev.realworldocaml.org/parsing-with-ocamllex-and-menhir.html *)
+and read_string buf =
+  parse
+  | '"'       { STRING (Buffer.contents buf) }
+  | '\\' '/'  { Buffer.add_char buf '/'; read_string buf lexbuf }
+  | '\\' '\\' { Buffer.add_char buf '\\'; read_string buf lexbuf }
+  | '\\' 'b'  { Buffer.add_char buf '\b'; read_string buf lexbuf }
+  | '\\' 'f'  { Buffer.add_char buf '\012'; read_string buf lexbuf }
+  | '\\' 'n'  { Buffer.add_char buf '\n'; read_string buf lexbuf }
+  | '\\' 'r'  { Buffer.add_char buf '\r'; read_string buf lexbuf }
+  | '\\' 't'  { Buffer.add_char buf '\t'; read_string buf lexbuf }
+  | [^ '"' '\\']+
+    { Buffer.add_string buf (Lexing.lexeme lexbuf);
+      read_string buf lexbuf
+    }
+  | _ { raise (SyntaxError ("Illegal string character: " ^ Lexing.lexeme lexbuf)) }
+  | eof { raise (SyntaxError ("String is not terminated")) }
