minuska/lib/libminuska.ml
@@ -1,5 +1,5 @@
-module Stringutils = Stringutils
-module Syntax = Syntax
+(*module Stringutils = Stringutils*)
+module Syntax = Libminuskapluginbase.Syntax
 module Micoqprint = Micoqprint
 module Miparse = Miparse
 module Miskeleton = Miskeleton
