minuska/lib/micoqprint.ml
@@ -1,29 +1,19 @@
+open Base
 open Core
+open Libminuskapluginbase
 open Syntax
 open Libminuskapluginbase.Pluginbase
-module Stringutils = Libminuskapluginbase.Stringutils
 
+(*
 type builtins_map_t = (string, string, String.comparator_witness) Map.t ;;
 type query_map_t = (string, string, String.comparator_witness) Map.t ;;
+*)
 
 let myiter (f : 'a -> 'b) (g : unit -> unit) (l : 'a list)  : unit =
     let ln = List.length l in
     List.iteri ~f:(fun idx x -> if (idx + 1 = ln) then (f x) else (f x; g ())) l;
     ()
-
-
-let output_part_2 = {delimiter|
-
-#[local]
-Instance LangDefaults : Defaults := {|
-    default_cseq_name := "builtin.cseq" ;
-    default_empty_cseq_name := "builtin.empty_cseq" ;
-    default_context_template := myContext ;
-
-    default_isValue := isValue ;
-|}.
-|delimiter}
-
+(*
 let translate_name
   (my_builtins_map : builtins_map_t)
   (my_query_map : query_map_t)
@@ -44,257 +34,195 @@ let translate_name
     | Some name1 ->
         let name = (name1) in
         ("e_fun", name)
+*)
+let rec groundterm_to_string
+    (pvae : primitiveValueAlgebraEntry)
+    (g : Syntax.groundterm)
+    : string =
+    match g with
+    | `GTb b -> (
+      (* sprintf "(@t_over string BuiltinRepr \"%s\")" (pvae.pvae_builtin_coq_quote b) *)
+      sprintf "(@t_over string BuiltinRepr {|br_kind:=\"%s\";br_value:=\"%s\"|})" (b.br_kind) (b.br_value)
+    )
+      | `GTerm (`Id s, gs) -> (
+      let gs_str = List.map ~f:(groundterm_to_string pvae) gs in
+      sprintf "(@t_term string BuiltinRepr \"%s\" %s)" s (Util.format_coq_string_list gs_str)
+      )
 
-let builtin2str (iface : 'a Extracted.builtinInterface) (name_of_builtins : coqModuleName) b =
-  (* This is only to throw error if we cannot convert it *)
-  let _ = Miskeleton.convert_builtin iface b in
-  let coq_entity = (get_primitive_value_algebra name_of_builtins).pvae_coq_entity_name in
-  match b with
-  | `BuiltinInt n -> "(bi_inject_Z _ "^coq_entity^" (fun a => match a with Some b => b | None => bi_inject_err _ "^(get_primitive_value_algebra name_of_builtins).pvae_coq_entity_name ^" end) (" ^ (string_of_int n) ^ ")%Z)"
-  | `BuiltinString s -> "(bi_inject_string _ "^coq_entity^" (fun a => match a with Some b => b | None => bi_inject_err _ "^(get_primitive_value_algebra name_of_builtins).pvae_coq_entity_name ^" end) \"" ^ s ^ "\")"
-  | _ -> failwith "Unsupported builtin value (for printing into Coq)"
-
-let rec print_groundterm
-  (oux : Out_channel.t)
-  (iface : 'a Extracted.builtinInterface)
-  (name_of_builtins : coqModuleName)
-  (g : Syntax.groundterm) : unit =
-  match g with
-  | `GTb b ->
-      fprintf oux "(@t_over symbol builtin_value ";
-      fprintf oux "%s" (builtin2str iface name_of_builtins b);
-      fprintf oux ")";
-  | `GTerm (`Id s, gs) ->
-    fprintf oux "(@t_term symbol builtin_value \"%s\" [" s;
-    myiter (fun x -> print_groundterm oux iface name_of_builtins x; ()) (fun () -> fprintf oux "; "; ()) gs;
-    fprintf oux "])"
-
-
-let rec print_resolved_w_hole
-  (oux : Out_channel.t)
-  (p : Syntax.pattern) (hole : string option) : unit =
+let rec pattern_w_hole_to_str
+  (pvae : primitiveValueAlgebraEntry)
+    (p : Syntax.pattern)
+    (hole : string option)
+    : string =
   match p with
   | `PVar (`Var s) -> (
       match hole with
-      | None ->
-          fprintf oux "(t_over (notations.inject_variable \"%s\"))" s
-      | Some s2 ->
-          if String.(s = s2) then
-              fprintf oux "(%s)" s2
-          else
-              fprintf oux "(t_over (notations.inject_variable \"%s\"))" s
-    )
-  | `PTerm (`Id s, ps) ->
-    fprintf oux "(@t_term _ _ \"%s\" [" s;
-    myiter (fun x -> print_resolved_w_hole oux x hole; ()) (fun () -> fprintf oux "; "; ()) ps;
-    fprintf oux "])"
+      | None -> (
+        sprintf "(t_over (sbov_var \"%s\"))" s
+      )
+      | Some s2 -> (
+        if String.(s=s2) then
+          sprintf "(%s)" s2
+        else
+          sprintf "(t_over (sbov_var \"%s\"))" s
+      )
+  )
+  | `PTerm (`Id s, ps) -> (
+    let ps_str = List.map ~f:(fun a -> pattern_w_hole_to_str pvae a hole) ps in
+    sprintf "(@t_term string StringBuiltinOrVar \"%s\" %s)" s (Util.format_coq_string_list ps_str)
+  )
 
-let rec print_pattern_w_hole (oux : Out_channel.t) (p : Syntax.pattern) (hole : string option) : unit =
-  match p with
-  | `PVar (`Var s) -> (
-      match hole with
-      | None ->
-          fprintf oux "(t_over (bov_variable \"%s\"))" s
-      | Some s2 ->
-          if String.(s = s2) then
-              fprintf oux "(%s)" s2
-          else
-              fprintf oux "(t_over (bov_variable \"%s\"))" s
-    )
-  | `PTerm (`Id s, ps) ->
-    fprintf oux "(@t_term symbol BuiltinOrVar \"%s\" [" s;
-    myiter (fun x -> print_pattern_w_hole oux x hole; ()) (fun () -> fprintf oux "; "; ()) ps;
-    fprintf oux "])"
+let pattern_to_str (pvae : primitiveValueAlgebraEntry) (p : Syntax.pattern) : string =
+  pattern_w_hole_to_str pvae p None
 
-let print_pattern (oux : Out_channel.t) (p : Syntax.pattern) : unit =
-  print_pattern_w_hole oux p None
-
-let rec print_expr_w_hole
-  (iface : 'a Extracted.builtinInterface)
-  (my_builtins_map : builtins_map_t)
-  (my_query_map : query_map_t)
-  (name_of_builtins : coqModuleName)
-  (oux : Out_channel.t)
+let rec expr_w_hole_to_str
+  (pvae : primitiveValueAlgebraEntry)
   (e : Syntax.expr)
   (hole : string option)
-  : unit =
+  : string
+  =
   match e with
   | `EVar (`Var s) -> (
-        match hole with
-        | None -> fprintf oux "(e_variable \"%s\")" s
-        | Some s2 ->
-            if String.(s = s2) then
-                fprintf oux "(%s)" s2
-            else
-                fprintf oux "(e_variable \"%s\")" s
-        )
-  | `EGround g ->
-    fprintf oux "(e_ground ";
-    print_groundterm oux iface name_of_builtins g;
-    fprintf oux ")"
+    match hole with
+    | None -> (
+      sprintf "(se_variable \"%s\")" s
+    )
+    | Some s2 -> (
+      if String.(s = s2) then (
+        sprintf "(%s)" s2
+      ) else (
+        sprintf "(se_variable \"%s\")" s
+      )
+    )
+  )
+  | `EGround g -> (
+    sprintf "(se_ground %s)" (groundterm_to_string pvae g)
+  )
+  | `ECallF (`Id s, es) -> (
+    let es_str = List.map ~f:(fun a -> expr_w_hole_to_str pvae a hole) es in
+    sprintf "(se_applyf \"%s\" %s)" s (Util.format_coq_string_list es_str)
+  )
+  | `ECallQ (`Id s, es) -> (
+    let es_str = List.map ~f:(fun a -> expr_w_hole_to_str pvae a hole) es in
+    sprintf "(se_applyq \"%s\" %s)" s (Util.format_coq_string_list es_str)
+  )
 
-  | `ECall (`Id s, es) ->
-    let (k, name) = translate_name my_builtins_map my_query_map s in
-    fprintf oux "(%s %s [" k name;
-    myiter (fun x -> print_expr_w_hole iface my_builtins_map my_query_map name_of_builtins oux x hole; ()) (fun () -> fprintf oux "; "; ()) es;
-    fprintf oux "])"
+  let expr_to_str (pvae : primitiveValueAlgebraEntry) (e : Syntax.expr) : string =
+    (expr_w_hole_to_str pvae e None)
 
+let rec exprterm_to_str
+    (pvae : primitiveValueAlgebraEntry)
+    (p : Syntax.exprterm)
+    : string =
+    match p with
+    | `EExpr e -> (
+      sprintf "(@t_over string StringExpression %s)" (expr_to_str pvae e)
+    )
+    | `ETerm (`Id s, ps) -> (
+      let ps_str = List.map ~f:(exprterm_to_str pvae) ps in
+      sprintf "(@t_term string StringExpression \"%s\" %s)" s (Util.format_coq_string_list ps_str)
+    )
 
-
-let print_expr
-  (iface : 'a Extracted.builtinInterface)
-  (my_builtins_map : builtins_map_t)
-  (my_query_map : query_map_t)
-  (name_of_builtins : coqModuleName)
-  (oux : Out_channel.t)
-  (e : Syntax.expr)
-  : unit =
-  print_expr_w_hole iface my_builtins_map my_query_map name_of_builtins oux e None
-
-let rec print_exprterm
-  (iface : 'a Extracted.builtinInterface)
-  (my_builtins_map : builtins_map_t)
-  (my_query_map : query_map_t)
-  (name_of_builtins : coqModuleName)
-  (oux : Out_channel.t)
-  (p : Syntax.exprterm)
-  : unit =
-  match p with
-  | `EExpr e -> fprintf oux "(@t_over symbol Expression2"; (print_expr iface my_builtins_map my_query_map name_of_builtins) oux e; fprintf oux ")";
-  | `ETerm (`Id s, ps) ->
-    fprintf oux "(@t_term symbol Expression2 \"%s\" [" s;
-    myiter (fun x -> print_exprterm iface my_builtins_map my_query_map name_of_builtins oux x; ()) (fun () -> fprintf oux "; "; ()) ps;
-    fprintf oux "])"
-
-let rec print_cond_w_hole
-  (iface : 'a Extracted.builtinInterface)
-  (my_builtins_map : builtins_map_t)
-  (my_query_map : query_map_t)
-  (name_of_builtins : coqModuleName)
-  (oux : Out_channel.t)
+let rec cond_w_hole_to_str
+  (pvae : primitiveValueAlgebraEntry)
   (c : Syntax.condition)
   (hole : string option)
-  : unit =
+  : string =
   match c with
-  | `CondAtomic (`Id s, es) ->
-      fprintf oux "(sc_atom %s [" (snd (translate_name my_builtins_map my_query_map s));
-      myiter (fun x -> print_expr_w_hole iface my_builtins_map my_query_map name_of_builtins oux x hole; ()) (fun () -> fprintf oux "; "; ()) es;
-      fprintf oux "])"
+  | `CondAtomic (`Id s, es) -> (
+    let es_str = List.map ~f:(fun a -> expr_w_hole_to_str pvae a hole) es in
+    sprintf "(ssc_atom \"%s\" %s)" s (Util.format_coq_string_list es_str)
+  )
   | `CondAnd (c1, c2) -> (
-    fprintf oux "(sc_and ";
-    print_cond_w_hole iface my_builtins_map my_query_map name_of_builtins oux c1 hole;
-    print_cond_w_hole iface my_builtins_map my_query_map name_of_builtins oux c2 hole;
-    fprintf oux ")";
-    ()
+    sprintf "(ssc_and %s %s)" (cond_w_hole_to_str pvae c1 hole) (cond_w_hole_to_str pvae c2 hole)
   )
   | `CondOr (c1, c2) -> (
-      fprintf oux "(sc_or ";
-      print_cond_w_hole iface my_builtins_map my_query_map name_of_builtins oux c1 hole;
-      print_cond_w_hole iface my_builtins_map my_query_map name_of_builtins oux c2 hole;
-      fprintf oux ")";
-      ()
+    sprintf "(ssc_or %s %s)" (cond_w_hole_to_str pvae c1 hole) (cond_w_hole_to_str pvae c2 hole)
   )
   | `CondTrue -> (
-    fprintf oux "sc_true";
-    ()
+    "ssc_true"
   )
   | `CondFalse -> (
-    fprintf oux "sc_false";
-    ()
+    "ssc_false"
   )
 
+let cond_to_str
+  (pvae : primitiveValueAlgebraEntry)
+    (c : Syntax.condition)
+    : string =
+    (cond_w_hole_to_str pvae c None)
+
+let rule_to_str
+    (pvae : primitiveValueAlgebraEntry)
+    (r : Syntax.rule)
+    : string =
+    let kind : string = (match r.frame with
+      | None -> (sprintf "basic_rule \"%s\"" (r.name))
+      | Some (`Id s) -> (
+        sprintf "framed_rule frame_%s \"%s\"" s (r.name)
+      )
+    ) in
+    sprintf "(%s %s %s %s)" kind (pattern_to_str pvae r.lhs) (exprterm_to_str pvae r.rhs) (cond_to_str pvae r.cond)
+
+let frame_to_str (pvae : primitiveValueAlgebraEntry) fr : string =
+  sprintf "(\"%s\",%s)" (match fr.fd_var with `Var s -> s) (pattern_to_str pvae fr.fd_pat)
+
+let frame_definition_to_str (pvae : primitiveValueAlgebraEntry) fr : string =
+  sprintf "Definition frame_%s : (string*(@TermOver' string StringBuiltinOrVar)) := %s.\n" (match fr.fd_name with `Id s -> s) (frame_to_str pvae fr)
+
+let decl_strict_to_str strictness : string = (
+  sprintf "(decl_strict Act (mkStrictnessDeclaration \"%s\" %d %s isValue myContext))\n"
+    (match strictness.symbol with `Id s -> s)
+    (strictness.arity)
+    (Util.format_coq_string_list (List.map ~f:(fun a -> sprintf "%d" a) strictness.strict_places))
+)
+
+let mycontext_decl_to_str (pvae : primitiveValueAlgebraEntry) ctx : string = (
+  let vname = (match (ctx.cd_var) with `Var s -> s) in
+  sprintf "Definition myContext := (fun (%s : @TermOver' string StringBuiltinOrVar) => %s).\n" vname (pattern_w_hole_to_str pvae (ctx.cd_pat) (Some vname))
+)
+
+let isvalue_decl_to_str (pvae : primitiveValueAlgebraEntry) value : string = (
+  let varname = (match (fst (value)) with `Var s -> s) in
+  sprintf "Definition isValue (%s : StringExpression) := %s.\n" varname (cond_w_hole_to_str pvae (snd value) (Some varname))
+)
 
 
-let print_rule
-  (iface : 'a Extracted.builtinInterface)
-  (my_builtins_map : builtins_map_t)
-  (my_query_map : query_map_t)
-  (name_of_builtins : coqModuleName)
-  (oux : Out_channel.t)
-  (r : Syntax.rule) : unit =
-    fprintf oux "(";
-    (
-      match (r.frame) with
-      | None -> 
-        fprintf oux "basic_rule my_program_info \"%s\" " (r.name)
-      | Some (`Id s) ->
-        fprintf oux "framed_rule my_program_info frame_%s \"%s\" " s (r.name)
-    );
-    
-    print_pattern oux (r.lhs);
-    fprintf oux " ";
-    print_exprterm iface my_builtins_map my_query_map name_of_builtins oux (r.rhs);
-    fprintf oux " ";
-    print_cond_w_hole iface my_builtins_map my_query_map name_of_builtins oux r.cond None;
-    (* fprintf oux "["; *)
-    (* myiter (fun x -> print_cond_w_hole iface my_builtins_map my_query_map name_of_builtins oux x None; ()) (fun () -> fprintf oux "; "; ()) (r.cond); *)
-    (* fprintf oux "]"; *)
-    fprintf oux ")\n";
-    ()
+let definition_to_str (pvae : primitiveValueAlgebraEntry) pi def : string = (
+  let builtins_import = (pvae.pvae_coq_import) in
+  let builtins_name = pvae.pvae_coq_entity_name in
+  sprintf
+{delimiter|
+Require Import Minuska.pval_ocaml_binding %s %s Minuska.default_everything.
+(* Definition mysignature := (bi_signature MyUnit %s). *)
+(* #[global] Existing Instance mysignature. *)
+(* Definition mybeta := (bi_beta MyUnit %s). *)
+(* #[global] Existing Instance mybeta. *)
+(* Definition my_program_info := %s. *)
+(* Definition mysigma : StaticModel := (default_everything.DSM my_program_info). *)
+(* #[global] Existing Instance mysigma. *)
+(* #[global] Existing Instance my_program_info. *)
+  %s
+  %s
+#[local]
+Instance LangDefaults : Defaults := mkDefaults "builtin.cseq" "builtin.empty_cseq" myContext isValue.
+  
+%s
+Definition Lang_Decls : list (Declaration Act) :=
+  (%s)
+  ++
+  (%s)
+. (* Lang_Decls *)
+|delimiter}
 
-let print_frame oux fr =
-  fprintf oux "Definition frame_%s : (variable*(TermOver BuiltinOrVar)) := (" (match fr.name with `Id s -> s);
-  fprintf oux "\"%s\"" (match fr.var with `Var s -> s);
-  fprintf oux ",";
-  print_pattern oux (fr.pat);
-  fprintf oux ").\n";
-  ()
-
-let print_strict oux str =
-  fprintf oux "(decl_strict (mkStrictnessDeclaration _ \"%s\" %d " (match str.symbol with `Id s -> s) (str.arity) ;
-  fprintf oux "[";
-  myiter (fun x -> fprintf oux "%d" x; ()) (fun () -> fprintf oux "; "; ()) (str.strict_places);
-  fprintf oux "] isValue _ myContext";
-  fprintf oux "))\n";
-  ()
-
-
-let print_mycontext oux ctx =
-  fprintf oux "Definition myContext := (context-template ";
-  print_resolved_w_hole oux (ctx.pat) (Some (match (ctx.var) with `Var s -> s));
-  fprintf oux " with %s).\n" (match ctx.var with `Var s -> s);
-  ()  
-
-
-let print_definition
-  (iface : 'a Extracted.builtinInterface)
-  (my_builtins_map : builtins_map_t)
-  (my_query_map : query_map_t)
-  ~(name_of_builtins : coqModuleName)
-  ~(name_of_pi : coqModuleName)
-  def oux =
-    let _ = def in
-    fprintf oux "Require Import Minuska.pval_ocaml_binding %s %s Minuska.default_everything.\n"  (get_primitive_value_algebra name_of_builtins).pvae_coq_import (get_pi name_of_pi).pie_coq_import;
-    fprintf oux "Definition mysignature := (bi_signature MyUnit %s).\n" (get_primitive_value_algebra name_of_builtins).pvae_coq_entity_name;
-    fprintf oux "#[global] Existing Instance mysignature.\n";
-    fprintf oux "Definition mybeta := (bi_beta MyUnit %s).\n" (get_primitive_value_algebra name_of_builtins).pvae_coq_entity_name;
-    fprintf oux "#[global] Existing Instance mybeta.\n";
-    fprintf oux "Definition my_program_info := %s.\n" (get_pi name_of_pi).pie_coq_entity_name;
-    fprintf oux "Definition mysigma : StaticModel := (default_everything.DSM my_program_info).\n";
-    fprintf oux "Existing Instance mysigma.\n";
-    (* fprintf oux "#[global] Existing Instance pi.%s.MyProgramInfo.\n" name_of_pi; *)
-    fprintf oux "#[global] Existing Instance my_program_info.\n";
-    print_mycontext oux (def.context);
-    
-    fprintf oux "Definition isValue (";
-    fprintf oux "%s" (match (fst (def.Syntax.value)) with `Var s -> s);
-    fprintf oux " : Expression2) := ";
-    print_cond_w_hole iface my_builtins_map my_query_map name_of_builtins oux (snd (def.Syntax.value)) (Some (match (fst (def.Syntax.value)) with `Var s -> s));
-    fprintf oux ".\n";
-    
-    fprintf oux "#[export] Instance isValue_nsc (X : Expression2) : NegableSideCondition (isValue X) := ltac:(intros; unfold isValue in *; apply _).\n";
-    
-    fprintf oux "%s\n" output_part_2;
-    List.iter ~f:(fun fr -> print_frame oux fr) (def.frames);
-    (* fprintf oux "%s\n" {|
-    Definition basic_rule (name : string) (l : TermOver BuiltinOrVar) (r : TermOver Expression2) (cond : Expression2) : Declaration :=
-      (decl_rule (@mkRuleDeclaration Extracted Act name (@mkRewritingRule2 Extracted Act l r [(mkSideCondition2 _ (e_nullary b_true) cond)] default_act)))
-    .
-    |}; *)
-    fprintf oux "Definition Lang_Decls : list Declaration := [\n";
-    myiter (fun x -> print_strict oux x; ()) (fun () -> fprintf oux ";" ; ()) (def.Syntax.strictness) ;
-    fprintf oux "%s" "] ++ [\n";
-    myiter (fun x -> print_rule iface my_builtins_map my_query_map (name_of_builtins : coqModuleName) oux x; ()) (fun () -> fprintf oux "; "; ()) (def.Syntax.rules);
-    fprintf oux "\n].\n";
-    ()
-    
+  builtins_import
+  (pi.pie_coq_import)
+  builtins_name
+  builtins_name
+  (pi.pie_coq_entity_name)
+  (mycontext_decl_to_str pvae (def.context))
+  (isvalue_decl_to_str pvae (def.Syntax.value))
+  (Util.format_string_list_per_line (List.map ~f:(frame_definition_to_str pvae) def.frames))
+  (Util.format_coq_string_list_per_line (List.map ~f:(decl_strict_to_str) def.Syntax.strictness))
+  (Util.format_coq_string_list_per_line (List.map ~f:(rule_to_str pvae) def.Syntax.rules))
+)
