minuska/lib/pluginbase.ml
@@ -1,7 +1,24 @@
-open Base
-open Core
 open Printf
 open Sexplib.Std
+
+type id = [ `Id of string ]
+
+type builtin_repr = {
+  br_kind : string ;
+  br_value : string;
+}
+
+(*
+type builtin =
+  [ `BuiltinInt of int
+  | `BuiltinString of string
+  | `BuiltinBool of bool
+  ]
+*)
+type groundterm =
+  [ `GTb of builtin_repr
+  | `GTerm of (id*(groundterm list))
+  ]
 
 type coqModuleName = 
 | User_module of string
@@ -14,13 +31,22 @@ type primitiveValueAlgebraEntry = {
   pvae_coq_import : string ;
   pvae_coq_entity_name : string ;
   pvae_builtin_interface : Dsm.__ Dsm.builtinInterface ;
+  pvae_builtin_inject : builtin_repr -> ((string, Dsm.__) Dsm.builtin_value) option ;
+  pvae_builtin_eject : (string, Dsm.__) Dsm.builtin_value -> builtin_repr option ;
+  pvae_builtin_coq_quote : builtin_repr -> string
 }
 
 type programInfoEntry = {
   pie_coq_import : string ;
   pie_coq_entity_name : string ;
-  pie_constructor : Dsm.__ -> (Dsm.__ Dsm.symbols) -> Dsm.__ -> Dsm.signature -> ((Dsm.__, Dsm.__) Dsm.model) -> (Dsm.__, Dsm.__) Dsm.programInfo ;
-  pie_table: (Dsm.string*Dsm.string) list ;
+  pie_constructor :
+    (* Dsm.__ -> *)
+    (* (Dsm.__ Dsm.symbols) -> *)
+    (* Dsm.__ -> *)
+    Dsm.signature ->
+    ((string, Dsm.__) Dsm.model) ->
+    (string, Dsm.__) Dsm.programInfo ;
+  pie_inject : string -> Dsm.__ option ;
 }
 
 (* private stuff *)
@@ -59,6 +85,50 @@ let get_primitive_value_algebra (primitive_value_algebra_name : coqModuleName) :
       pvae_coq_import = "Minuska.builtin."^name;
       pvae_builtin_interface = m;
       pvae_coq_entity_name = (sprintf "builtins_%s" name);
+      pvae_builtin_inject = (fun (b : builtin_repr) -> (
+        Stdlib.Obj.magic (
+        match name with
+        | "klike" -> (
+          match b.br_kind with
+          | "int" -> (Option.some (Dsm.Bv_Z (Z.of_string (b.br_value))))
+          | "bool" -> (
+            match b.br_value with
+            | "true" -> (Option.some (Dsm.Bv_bool true))
+            | "false" -> (Option.some (Dsm.Bv_bool false))
+            | _ -> failwith (sprintf "Unknown boolean value '%s': only 'true' and 'false' are allowed" b.br_value)
+          )
+          | "string" -> (Option.some (Dsm.Bv_str ((*Stringutils.explode*) b.br_value)))
+          | _ -> failwith (sprintf "Unknown kind of builtins: '%s'" b.br_kind)
+        )
+        | _ -> failwith (sprintf "Cannot represent given builtin using module '%s'" name)
+      )
+      ));
+      pvae_builtin_coq_quote = (fun (b : builtin_repr) -> (
+        Stdlib.Obj.magic (
+        match name with
+        | "klike" -> (
+          match b.br_kind with
+          | "int" -> (sprintf "(bv_Z (%s)%%Z)" (b.br_value))
+          | "bool" -> (
+            match b.br_value with
+            | "true" -> ("(bv_bool true)")
+            | "false" -> ("(bv_bool false)")
+            | _ -> failwith (sprintf "Unknown boolean value '%s': only 'true' and 'false' are allowed" b.br_value)
+          )
+          | "string" -> (sprintf "(bv_str \"%s\")" b.br_value)
+          | _ -> failwith (sprintf "Unknown kind of builtins: '%s'" b.br_kind)
+        )
+        | _ -> failwith (sprintf "Cannot represent given builtin using module '%s'" name)
+      )
+      ));
+      pvae_builtin_eject = (fun b -> (match (Stdlib.Obj.magic b) with
+        | Dsm.Bv_Z z -> (Option.some ({br_kind="int"; br_value=(Z.to_string z);}))
+        | Dsm.Bv_bool b' -> (Option.some ({br_kind="bool"; br_value=(if b' then "true" else "false");}))
+        | Dsm.Bv_str s -> (Option.some (({br_kind="string"; br_value=s};)))
+        | Dsm.Bv_list _ -> (Option.some {br_kind="list"; br_value="_"})
+        | Dsm.Bv_pmap _ -> (Option.some {br_kind="map"; br_value="_"})
+        (* | _ -> Option.none *)
+      ));
     }
   )
   | User_module name -> (
@@ -74,7 +144,7 @@ let get_pi (program_info_name : coqModuleName) : programInfoEntry
       | "trivial" -> Dsm.pi_trivial
       | _ -> failwith (sprintf "Unknown program info specified: '%s'" name)
     ) in
-    ({ pie_constructor = (fst m); pie_table = (snd m); pie_coq_import = (sprintf "Minuska.pi.%s" name); pie_coq_entity_name = (sprintf "%s.MyProgramInfo" name)})
+    ({ pie_constructor = (fst m); pie_inject = (fun s -> Obj.magic ((snd m) s)); pie_coq_import = (sprintf "Minuska.pi.%s" name); pie_coq_entity_name = (sprintf "%s.MyProgramInfo" name)})
   )
   | User_module name -> (
       Hashtbl.find programInfoEntries name
