minuska/lib/util.ml
@@ -1,0 +1,21 @@
+open Core
+open Printf
+
+let format_string_list0 (open_br : string) (close_br: string) (sep : string) (l : string list) : string =
+  match l with
+  | [] -> (sprintf "%s%s" open_br close_br)
+  | x::[] -> (sprintf "%s %s %s" open_br x close_br)
+  | x::y::zs ->
+    (sprintf "%s %s%s %s" open_br x (List.fold_left ~init:("") ~f:(fun b a -> sprintf "%s%s%s" b sep a) (y::zs)) close_br )
+
+let format_string_list (l : string list) : string =
+  (format_string_list0 "[" "]" ", " l)
+
+let format_coq_string_list (l : string list) : string =
+  (format_string_list0 "[" "]" "; " l)
+
+let format_coq_string_list_per_line (l : string list) : string =
+  (format_string_list0 "[" "]" ";\n" l)
+
+let format_string_list_per_line (l : string list) : string =
+  (format_string_list0 "" "" "\n" l)
