coq-minuska/theories/builtin/klike.v
@@ -90,7 +90,7 @@ Section sec.
 
     (* TODO make parametric in a user type *)
     Inductive BuiltinValue0 :=
-    | bv_error
+    (* | bv_error *)
     | bv_bool (b : bool)
     (* | bv_nat (n : nat) *)
     | bv_Z (z : Z)
@@ -162,7 +162,7 @@ Section sec.
     end) in
         S (my_pmapne_size m)
     | bv_pmap (PEmpty) => 1
-    | bv_error => 1
+    (* | bv_error => 1 *)
     | bv_bool _ => 1
     (* | bv_nat _ => 1 *)
     | bv_sym _ => 1
@@ -185,11 +185,11 @@ Section sec.
         }
         {
             destruct x.
-            {
+            (* {
                 destruct y;
                 try (solve [left; reflexivity]);
                 right; ltac1:(discriminate).
-            }
+            } *)
             {
                 destruct y;
                 try (solve [left; reflexivity]);
@@ -932,7 +932,7 @@ Section sec.
     Defined.
 
     Inductive BVLeaf :=
-    | bvl_error
+    (* | bvl_error *)
     | bvl_bool (b : bool)
     (* | bvl_nat (n : nat) *)
     | bvl_Z (z : Z)
@@ -950,7 +950,7 @@ Section sec.
         (t : gen_tree BVLeaf) : (option BuiltinValue0)  :=
     match t with
     | ((GenNode 1 nil)) => Some (bv_pmap (PEmpty))
-    | (GenLeaf bvl_error)      => Some (bv_error)  
+    (* | (GenLeaf bvl_error)      => Some (bv_error)   *)
     | (GenLeaf (bvl_bool b))   => Some (bv_bool b)
     (* | (GenLeaf (bvl_nat n))    => Some (bv_nat n)  *)
     | (GenLeaf (bvl_Z z))      => Some (bv_Z z) 
@@ -1136,7 +1136,7 @@ Section sec.
         (r : BuiltinValue0) : (gen_tree BVLeaf) :=
     match r with
     | (bv_pmap (PEmpty)) => (GenNode 1 nil)
-    | (bv_error)         => (GenLeaf bvl_error)
+    (* | (bv_error)         => (GenLeaf bvl_error) *)
     | (bv_bool b)        => (GenLeaf (bvl_bool b))
     (* | (bv_nat n)         => (GenLeaf (bvl_nat n)) *)
     | (bv_Z z)           => (GenLeaf (bvl_Z z))
@@ -1571,7 +1571,7 @@ induction ao; try reflexivity.
     )).
     {
         ltac1:(unshelve(eapply gen_tree_countable)).
-        remember (unit+bool+(*nat+*)Z+string+symbol)%type as MyT.
+        remember ((*unit+*)bool+(*nat+*)Z+string+symbol)%type as MyT.
         ltac1:(unshelve(eapply @inj_countable with (A := MyT))).
         {
             subst MyT. apply _.
@@ -1580,10 +1580,7 @@ induction ao; try reflexivity.
             subst.
             intros bvl. destruct bvl.
             {
-                left. left. left. left. exact ().
-            }
-            {
-                left. left. left. right. exact b.
+                left. left. left. exact b.
             }
             {
                 left. left. right. exact z.
@@ -1604,15 +1601,15 @@ induction ao; try reflexivity.
                 {
                     destruct t1 as [t1|t2].
                     {
-                        destruct t1 as [t1|t2].
+                        (* destruct t1 as [t1|t2].
                         {
                             apply Some.
                             apply bvl_error.
-                        }
+                        } *)
                         {
                             apply Some.
                             apply bvl_bool.
-                            apply t2.
+                            apply t1.
                         }
                     }
                     {
@@ -1704,11 +1701,10 @@ Qed.
 Fail Next Obligation.
 
 Inductive PredicateSymbol : Set :=
-| b_tt                     (* Prop *)
 | b_isBuiltin              (* 'a -> Prop *)
 | b_isNotBuiltin           (* 'a -> Prop *)
-| b_isError                (* 'a -> Prop *)
-| b_isNotError             (* 'a -> Prop *)
+(*| b_isError                (* 'a -> Prop *)*)
+(*| b_isNotError             (* 'a -> Prop *)*)
 | b_isSymbol               (* 'a -> Prop *)
 | b_isNotSymbol            (* 'a -> Prop *)
 | b_isZ                    (* 'a -> Prop *)
@@ -1739,11 +1735,10 @@ Proof. ltac1:(solve_decision). Defined.
 #[export]
 Program Instance PredicateSymbol_fin : Finite PredicateSymbol := {|
     enum := [
-        b_tt                     ;
         b_isBuiltin              ;
         b_isNotBuiltin           ;
-        b_isError                ;
-        b_isNotError             ;
+        (* b_isError                ;
+        b_isNotError             ; *)
         b_isSymbol               ;
         b_isNotSymbol            ;
         b_isZ                    ;
@@ -1784,16 +1779,6 @@ Section sec2.
 
     Definition BuiltinValue := @BuiltinValue0 symbol.
 
-    Definition err
-    :=
-        @t_over symbol BuiltinValue bv_error
-    .
-
-    Definition impl_isError (bv : BuiltinValue) : bool
-    :=
-        match bv with bv_error => true | _ => false end
-    .
-
     Definition impl_isZ (bv : BuiltinValue) : bool
     :=
         match bv with bv_Z _ => true | _ => false end
@@ -1820,23 +1805,23 @@ Section sec2.
     .
 
     Definition bfmap1
-        (f : BuiltinValue -> BuiltinValue)
+        (f : BuiltinValue -> option BuiltinValue)
         (x : @TermOver' symbol BuiltinValue)
-        : @TermOver' symbol BuiltinValue
+        : option (@TermOver' symbol BuiltinValue)
     :=
     match x with
-    | t_over x' => t_over (f x')
-    | _ => err
+    | t_over x' => t_over <$> (f x')
+    | _ => None
     end.
 
     Definition bfmap2
-        (f : BuiltinValue -> BuiltinValue -> BuiltinValue)
+        (f : BuiltinValue -> BuiltinValue -> option BuiltinValue)
         (x y : @TermOver' symbol BuiltinValue)
-        : @TermOver' symbol BuiltinValue
+        : option (@TermOver' symbol BuiltinValue)
     :=
     match x, y with
-    | t_over x', t_over y' => t_over (f x' y')
-    | _,_ => err
+    | t_over x', t_over y' => (t_over <$> (f x' y'))
+    | _,_ => None
     end.
 
     Definition bfmap2P
@@ -1852,13 +1837,13 @@ Section sec2.
     Definition bfmap_Z_Z__Z
         (f : Z -> Z -> Z)
         (x y : @TermOver' symbol BuiltinValue)
-        : @TermOver' symbol BuiltinValue
+        : option (@TermOver' symbol BuiltinValue)
     :=
     bfmap2
         (fun x' y' =>
         match x', y' with
-        | bv_Z x'', bv_Z y'' => bv_Z (f x'' y'')
-        | _, _ => bv_error
+        | bv_Z x'', bv_Z y'' => Some (bv_Z (f x'' y''))
+        | _, _ => None
         end
         )
         x y
@@ -1882,119 +1867,180 @@ Section sec2.
     Definition bfmap_Z_Z__bool
         (f : Z -> Z -> bool)
         (x y : @TermOver' symbol BuiltinValue)
-        : @TermOver' symbol BuiltinValue
+        : option (@TermOver' symbol BuiltinValue)
     :=
     bfmap2
         (fun x' y' =>
         match x', y' with
-        | bv_Z x'', bv_Z y'' => bv_bool (f x'' y'')
-        | _, _ => bv_bool false
+        | bv_Z x'', bv_Z y'' => Some (bv_bool (f x'' y''))
+        | _, _ => Some (bv_bool false)
         end
         )
         x y
     .
 
     Definition my_encode := ((@encode (@TermOver' (symbol) BuiltinValue0)) _ (@TermOver_countable (symbol) BuiltinValue0 (@symbol_eqdec symbol symbols) _ (@symbol_countable symbol symbols) (@BuiltinValue0_countable (symbol) (@symbol_eqdec symbol symbols) (@symbol_countable symbol symbols)))).
+    Definition my_decode := ((@decode (@TermOver' (symbol) BuiltinValue0)) _ (@TermOver_countable (symbol) BuiltinValue0 (@symbol_eqdec symbol symbols) _ (@symbol_countable symbol symbols) (@BuiltinValue0_countable (symbol) (@symbol_eqdec symbol symbols) (@symbol_countable symbol symbols)))).
 
 
     Definition liftNulary
-        (f : MyUnit -> (@TermOver' (symbol) BuiltinValue))
-        : (MyUnit -> list (@TermOver' (symbol) BuiltinValue) -> (@TermOver' (symbol) BuiltinValue))
+        (f : MyUnit -> option (@TermOver' (symbol) BuiltinValue))
+        : (MyUnit -> list (@TermOver' (symbol) BuiltinValue) -> option (@TermOver' (symbol) BuiltinValue))
     :=
         fun nv l =>
         match l with
         | [] => f nv
-        | _::_ => @t_over symbol BuiltinValue (bv_error)
+        | _::_ => None
         end
     .
 
     Definition liftNularyP
-        (f : MyUnit -> bool)
-        : (MyUnit -> list (@TermOver' (symbol) BuiltinValue) -> bool)
+        (f : MyUnit -> option bool)
+        : (MyUnit -> list (@TermOver' (symbol) BuiltinValue) -> option bool)
     :=
         fun nv l =>
         match l with
         | [] => f nv
-        | _::_ => false
+        | _::_ => None
         end
     .
 
     Definition liftUnary
-        (f : MyUnit -> (@TermOver' (symbol) BuiltinValue) -> (@TermOver' (symbol) BuiltinValue))
-        : (MyUnit -> list (@TermOver' (symbol) BuiltinValue) -> (@TermOver' (symbol) BuiltinValue))
+        (f : MyUnit -> (@TermOver' (symbol) BuiltinValue) -> option (@TermOver' (symbol) BuiltinValue))
+        : (MyUnit -> list (@TermOver' (symbol) BuiltinValue) -> option (@TermOver' (symbol) BuiltinValue))
     :=
         fun nv l =>
         match l with
-        | [] => @t_over symbol BuiltinValue (bv_error)
+        | [] => None
         | x1::[] => f nv x1
-        | _::_::_ => @t_over symbol BuiltinValue (bv_error)
+        | _::_::_ => None
         end
     .
 
     Definition liftUnaryP
-        (f : MyUnit -> (@TermOver' (symbol) BuiltinValue) -> bool)
-        : (MyUnit -> list (@TermOver' (symbol) BuiltinValue) -> bool)
+        (f : MyUnit -> (@TermOver' (symbol) BuiltinValue) -> option bool)
+        : (MyUnit -> list (@TermOver' (symbol) BuiltinValue) -> option bool)
     :=
         fun nv l =>
         match l with
-        | [] => false
+        | [] => None
         | x1::[] => f nv x1
-        | _::_::_ => false
+        | _::_::_ => None
         end
     .
 
     Definition liftBinary
-        (f : MyUnit -> (@TermOver' (symbol) BuiltinValue) -> (@TermOver' (symbol) BuiltinValue) -> (@TermOver' (symbol) BuiltinValue))
-        : (MyUnit -> list (@TermOver' (symbol) BuiltinValue) -> (@TermOver' (symbol) BuiltinValue))
+        (f : MyUnit -> (@TermOver' (symbol) BuiltinValue) -> (@TermOver' (symbol) BuiltinValue) -> option (@TermOver' (symbol) BuiltinValue))
+        : (MyUnit -> list (@TermOver' (symbol) BuiltinValue) -> option (@TermOver' (symbol) BuiltinValue))
     :=
         fun nv l =>
         match l with
-        | [] => @t_over symbol BuiltinValue (bv_error)
-        | _::[] => @t_over symbol BuiltinValue (bv_error)
+        | [] => None
+        | _::[] => None
         | x1::x2::[] => f nv x1 x2
-        | _::_::_::_ => @t_over symbol BuiltinValue (bv_error)
+        | _::_::_::_ => None
         end
     .
 
     Definition liftBinaryP
-        (f : MyUnit -> (@TermOver' (symbol) BuiltinValue) -> (@TermOver' (symbol) BuiltinValue) -> bool)
-        : (MyUnit -> list (@TermOver' (symbol) BuiltinValue) -> bool)
+        (f : MyUnit -> (@TermOver' (symbol) BuiltinValue) -> (@TermOver' (symbol) BuiltinValue) -> option bool)
+        : (MyUnit -> list (@TermOver' (symbol) BuiltinValue) -> option bool)
     :=
         fun nv l =>
         match l with
-        | [] => false
-        | _::[] => false
+        | [] => None
+        | _::[] => None
         | x1::x2::[] => f nv x1 x2
-        | _::_::_::_ => false
+        | _::_::_::_ => None
         end
     .
 
     Definition liftTernary
-        (f : MyUnit -> (@TermOver' (symbol) BuiltinValue) -> (@TermOver' (symbol) BuiltinValue) -> (@TermOver' (symbol) BuiltinValue) -> (@TermOver' (symbol) BuiltinValue))
-        : (MyUnit -> list (@TermOver' (symbol) BuiltinValue) -> (@TermOver' (symbol) BuiltinValue))
+        (f : MyUnit -> (@TermOver' (symbol) BuiltinValue) -> (@TermOver' (symbol) BuiltinValue) -> (@TermOver' (symbol) BuiltinValue) -> option (@TermOver' (symbol) BuiltinValue))
+        : (MyUnit -> list (@TermOver' (symbol) BuiltinValue) -> option (@TermOver' (symbol) BuiltinValue))
     :=
         fun nv l =>
         match l with
-        | [] => @t_over symbol BuiltinValue (bv_error)
-        | _::[] => @t_over symbol BuiltinValue (bv_error)
-        | _::_::[] => @t_over symbol BuiltinValue (bv_error)
+        | [] => None
+        | _::[] => None
+        | _::_::[] => None
         | x1::x2::x3::[] => f nv x1 x2 x3
-        | _::_::_::_::_ => @t_over symbol BuiltinValue (bv_error)
+        | _::_::_::_::_ => None
         end
     .
 
     #[local]
-    Instance mysignature : Signature := {|
+    Program Instance mysignature : Signature := {|
         builtin_function_symbol
             := FunctionSymbol ;
 
         builtin_predicate_symbol
             := PredicateSymbol ;
     
+        bps_ar := fun p =>
+            match p with
+            | b_isBuiltin => 1
+            | b_isNotBuiltin => 1
+            | b_isSymbol => 1
+            | b_isNotSymbol => 1
+            | b_isZ => 1
+            | b_isNotZ => 1
+            | b_isBool => 1
+            | b_isNotBool => 1
+            | b_isString => 1
+            | b_isNotString => 1
+            | b_isList => 1
+            | b_isNotList => 1
+            | b_isMap => 1
+            | b_isNotMap => 1
+            | b_bool_is_true => 1
+            | b_bool_is_false => 1
+            | b_term_eq => 2
+            | b_map_hasKey => 2
+            | b_is_applied_symbol => 2
+            | b_is_not_applied_symbol => 2
+            | b_have_same_symbol => 2
+            | b_have_different_symbols => 2
+            end ;
+        bps_neg := fun p =>
+            match p with
+            | b_isBuiltin => Some b_isNotBuiltin
+            | b_isNotBuiltin => Some b_isBuiltin
+            | b_isSymbol => Some b_isNotSymbol
+            | b_isNotSymbol => Some b_isSymbol
+            | b_isZ => Some b_isNotZ
+            | b_isNotZ => Some b_isZ
+            | b_isBool => Some b_isNotBool
+            | b_isNotBool => Some b_isBool
+            | b_isString => Some b_isNotString
+            | b_isNotString => Some b_isString
+            | b_isList => Some b_isNotList
+            | b_isNotList => Some b_isList
+            | b_isMap => Some b_isNotMap
+            | b_isNotMap => Some b_isMap
+            | b_bool_is_true => Some b_bool_is_false
+            | b_bool_is_false => Some b_bool_is_true
+            | b_term_eq => None
+            | b_map_hasKey => None
+            | b_is_applied_symbol => Some b_is_not_applied_symbol
+            | b_is_not_applied_symbol => Some b_is_applied_symbol
+            | b_have_same_symbol => Some b_have_different_symbols
+            | b_have_different_symbols => Some b_have_same_symbol
+            end ;
+
     |}.
+    Next Obligation.
+        intros p p' H; destruct p, p'; ltac1:(simplify_eq/=); reflexivity.
+    Qed.
+    Next Obligation.
+        intros p p' H; destruct p; simpl; ltac1:(simplify_eq/=); try reflexivity.
+    Qed.
+    Fail Next Obligation.
 
     #[local]
-    Instance βover
+    Obligation Tactic := Program.Tactics.program_simpl.
+    Program
+    Definition βover
         : ModelOver mysignature MyUnit BuiltinValue0
     := {|
 
@@ -2003,27 +2049,27 @@ Section sec2.
             match p with
             (* nulary *)
             | b_zero => liftNulary (
-                    fun _ => t_over (bv_Z 0)
+                    fun _ => Some (t_over (bv_Z 0))
                 )
             | b_list_empty =>  liftNulary (
-                    fun _ => (t_over (bv_list nil))
+                    fun _ => Some ((t_over (bv_list nil)))
                 )
             | b_map_empty =>  liftNulary (
-                    fun _ => (t_over (bv_pmap ∅))
+                    fun _ => Some (t_over (bv_pmap ∅))
                 )
             (* unary *)            
             | b_bool_neg => liftUnary (
                 fun _ v =>
                 match v with
-                | t_over (bv_bool b) => t_over (bv_bool (negb b))
-                | _ => err
+                | t_over (bv_bool b) => Some (t_over (bv_bool (negb b)))
+                | _ => None
                 end
             )
             | b_map_size => liftUnary (
                 fun _ v =>
                 match v with
-                | t_over (bv_pmap m) => (t_over (bv_Z (Z.of_nat (size m))))
-                | _ => err
+                | t_over (bv_pmap m) => Some (t_over (bv_Z (Z.of_nat (size m))))
+                | _ => None
                 end
             )
             | b_Z_plus => liftBinary (
@@ -2041,19 +2087,19 @@ Section sec2.
             | b_Z_div => liftBinary (
                 fun _ v1 v2 =>
                 match v2 with
-                | t_over (bv_Z (0)) => err
+                | t_over (bv_Z (0)) => None
                 | _ => bfmap_Z_Z__Z Z.div v1 v2
                 end
             )
 
             | b_Z_eq => liftBinary (
                 fun _ v1 v2 =>
-                t_over (bv_bool (bool_decide (v1 = v2)))
+                Some (t_over (bv_bool (bool_decide (v1 = v2))))
             )
 
             | b_Z_neq => liftBinary (
                 fun _ v1 v2 =>
-                t_over (bv_bool (negb (bool_decide (v1 = v2))))
+                Some (t_over (bv_bool (negb (bool_decide (v1 = v2)))))
             )
 
             | b_Z_isLe => liftBinary (
@@ -2082,10 +2128,10 @@ Section sec2.
                 | t_over (bv_pmap m) =>
                     let p := my_encode (v2) in
                     match m !! p with
-                    | Some v => (prettify v)
-                    | None => err
+                    | Some v => Some (prettify v)
+                    | None => None
                     end
-                | _ => err
+                | _ => None
                 end
             )
 
@@ -2096,8 +2142,8 @@ Section sec2.
                 | t_over (bv_pmap m) =>
                     let p := my_encode (v2) in
                     let m' := <[ p := (uglify' v3) ]>m in
-                    t_over (bv_pmap m')
-                | _ => err
+                    Some (t_over (bv_pmap m'))
+                | _ => None
                 end
             )
             end ;
@@ -2105,153 +2151,134 @@ Section sec2.
             builtin_predicate_interp
             := fun p =>
             match p with
-            | b_tt => liftNularyP (
-                fun _ =>
-                true
-            )
             | b_term_eq => liftBinaryP (
                 fun _ v1 v2 =>
-                (bool_decide (v1 = v2))
+                Some (bool_decide (v1 = v2))
             )
 
             | b_bool_is_true => liftUnaryP (
                 fun _ v =>
                 match v with
-                | t_over (bv_bool b) => eqb b true
-                | _ => false
+                | t_over (bv_bool b) => Some (eqb b true)
+                | _ => None
                 end
             )
 
             | b_bool_is_false => liftUnaryP (
                 fun _ v =>
                 match v with
-                | t_over (bv_bool b) => eqb b false
-                | _ => false
+                | t_over (bv_bool b) => Some (eqb b false)
+                | _ => None
                 end
             )
 
             | b_isBuiltin => liftUnaryP (
                 fun _ v =>
                 match v with
-                | t_over b => true
-                | t_term _ _ => false
+                | t_over b => Some true
+                | t_term _ _ => Some false
                 end
             )
             | b_isNotBuiltin => liftUnaryP (
                 fun _ v =>
                 match v with
-                | t_over b => false
-                | t_term _ _ => true
-                end
-            ) 
-            | b_isError => liftUnaryP (
-                fun _ v =>
-                match v with
-                | t_over x => (impl_isError x)
-                | _ => false
+                | t_over b => Some false
+                | t_term _ _ => Some true
                 end
             )
-            | b_isNotError => liftUnaryP (
-                fun _ v =>
-                match v with
-                | t_over x => negb (impl_isError x)
-                | _ => false
-                end
-            )
-
             | b_isSymbol => liftUnaryP (
                 fun _ v =>
                 match v with
-                | t_term _ _ => true
-                | _ => false
+                | t_term _ _ => Some true
+                | _ => Some false
                 end
             )
 
             | b_isNotSymbol => liftUnaryP (
                 fun _ v =>
                 match v with
-                | t_term _ _ => false
-                | _ => true
+                | t_term _ _ => Some false
+                | _ => Some true
                 end
             )
    
             | b_isString => liftUnaryP (
                 fun _ v =>
                 match v with
-                | t_over x => (impl_isString x)
-                | _ => false
+                | t_over x => Some (impl_isString x)
+                | _ => Some false
                 end
             )
 
             | b_isNotString => liftUnaryP (
                 fun _ v =>
                 match v with
-                | t_over x => negb (impl_isString x)
-                | _ => true
+                | t_over x => Some (negb (impl_isString x))
+                | _ => Some true
                 end
             )
                 
             | b_isList => liftUnaryP (
                 fun _ v =>
                 match v with
-                | t_over x => (impl_isList x)
-                | _ => false
+                | t_over x => Some (impl_isList x)
+                | _ => Some false
                 end
             )
 
             | b_isNotList => liftUnaryP (
                 fun _ v =>
                 match v with
-                | t_over x => negb (impl_isList x)
-                | _ => true
+                | t_over x => Some (negb (impl_isList x))
+                | _ => Some true
                 end
             )
 
             | b_isBool => liftUnaryP (
                 fun _ v =>
                 match v with
-                | t_over x => (impl_isBool x)
-                | _ => false
+                | t_over x => Some (impl_isBool x)
+                | _ => Some false
                 end
             )
 
             | b_isNotBool => liftUnaryP (
                 fun _ v =>
                 match v with
-                | t_over x => negb (impl_isBool x)
-                | _ => true
+                | t_over x => Some (negb (impl_isBool x))
+                | _ => Some true
                 end
             )
                 
             | b_isMap => liftUnaryP (
                 fun _ v =>
                 match v with
-                | t_over x => (impl_isMap x)
-                | _ => false
+                | t_over x => Some (impl_isMap x)
+                | _ => Some false
                 end
             )
 
             | b_isNotMap => liftUnaryP (
                 fun _ v =>
                 match v with
-                | t_over x => negb (impl_isMap x)
-                | _ => true
+                | t_over x => Some (negb (impl_isMap x))
+                | _ => Some true
                 end
             )
 
             | b_isZ => liftUnaryP (
                 fun _ v =>
                 match v with
-                | t_over x => (impl_isZ x)
-                | _ => false
+                | t_over x => Some (impl_isZ x)
+                | _ => Some false
                 end
             )
 
             | b_isNotZ => liftUnaryP (
                 fun _ v =>
                 match v with
-                | t_over x => negb (impl_isZ x)
-                | _ => true
+                | t_over x => Some (negb (impl_isZ x))
+                | _ => Some true
                 end
             )    
 
@@ -2261,10 +2288,10 @@ Section sec2.
                 | t_over (bv_pmap m) =>
                     let p := my_encode (v2) in
                     match m !! p with
-                    | Some _ => true
-                    | None => false
+                    | Some _ => Some true
+                    | None => Some false
                     end
-                | _ => false
+                | _ => None
                 end
             )
 
@@ -2273,10 +2300,10 @@ Section sec2.
                 match v1 with
                 | t_term s1 _ =>
                     match v2 with
-                    | t_term s2 _ => (bool_decide (s1 = s2))
-                    | _ => false
+                    | t_term s2 _ => Some (bool_decide (s1 = s2))
+                    | _ => Some false
                     end
-                | _ => false
+                | _ => Some false
                 end
             )
 
@@ -2285,10 +2312,10 @@ Section sec2.
                 match v1 with
                 | t_term s1 _ =>
                     match v2 with
-                    | t_term s2 _ => negb (bool_decide (s1 = s2))
-                    | _ => false
+                    | t_term s2 _ => Some (negb (bool_decide (s1 = s2)))
+                    | _ => Some true
                     end
-                | _ => false
+                | _ => Some true
                 end
             )
 
@@ -2297,10 +2324,10 @@ Section sec2.
                 match v1 with
                 | t_over (bv_sym s) =>
                     match v2 with
-                    | t_term s' _ => (bool_decide (s' = s))
-                    | _ => false
+                    | t_term s' _ => Some (bool_decide (s' = s))
+                    | _ => None
                     end
-                | _ => false
+                | _ => None
                 end
             )
 
@@ -2309,14 +2336,49 @@ Section sec2.
                 match v1 with
                 | t_over (bv_sym s) =>
                     match v2 with
-                    | t_term s' _ => negb (bool_decide (s' = s))
-                    | _ => true
+                    | t_term s' _ => Some ( negb (bool_decide (s' = s)))
+                    | _ => None
                     end
-                | _ => true
+                | _ => None
                 end
             )
             end ;
+            bps_neg_correct := _;
     |}.
+    (* Solve All Obligations with (simpl; intros; try discriminate). *)
+    (* Fail Next Obligation. *)
+    Next Obligation.
+        intros.
+        destruct p,p'; simpl in *; case_on_length (); ltac1:(repeat case_match; simplify_eq/=); try reflexivity.
+        {
+          rewrite negb_involutive. reflexivity.
+        }
+        {
+          rewrite negb_involutive. reflexivity.
+        }
+        {
+          rewrite negb_involutive. reflexivity.
+        }
+        {
+          rewrite negb_involutive. reflexivity.
+        }
+        {
+          rewrite negb_involutive. reflexivity.
+        }
+        {
+          destruct b0; reflexivity.
+        }
+        {
+          destruct b0; reflexivity.
+        }
+        {
+          rewrite negb_involutive. reflexivity.
+        }
+        {
+          rewrite negb_involutive. reflexivity.
+        }
+    Qed.
+    Fail Next Obligation.
 
     #[local]
     Instance β
@@ -2328,79 +2390,38 @@ Section sec2.
         builtin_model_over := βover ;
     |}.
 
+
+    Definition sym_info : string -> SymbolInfo :=
+    fun s => match s with
+    | "sym.is" => si_predicate b_isSymbol 1 (Some "sym.isNot")
+    | "sym.isNot" => si_predicate b_isNotSymbol 1 (Some "sym.is")
+    | "bool.is" => si_predicate b_isBool 1 (Some "bool.isNot")
+    | "bool.isNot" => si_predicate b_isNotBool 1 (Some "bool.is")
+    | "string.is" => si_predicate b_isString 1 (Some "string.isNot")
+    | "string.isNot" => si_predicate b_isNotString 1 (Some "string.is")
+    | "z.is" => si_predicate b_isZ 1 (Some "z.isNot")
+    | "z.isNot" => si_predicate b_isNotZ 1 (Some "z.is")
+    | "bool.neg" => si_function b_bool_neg
+    | "bool.is_true" => si_predicate b_bool_is_true 1 (Some "bool.is_false")
+    | "bool.is_false" => si_predicate b_bool_is_false 1 (Some "bool.is_true")
+    | "term.eq" => si_predicate b_term_eq 2 None
+    | "term.same_symbol" => si_predicate b_have_same_symbol 2 (Some "term.different_symbol")
+    | "term.different_symbol" => si_predicate b_have_different_symbols 2 (Some "term.same_symbol")
+    | "z.plus" => si_function b_Z_plus
+    | "z.minus" => si_function b_Z_minus
+    | "z.eq" => si_function b_Z_eq
+    | "z.le" => si_function b_Z_isLe
+    | "z.lt" => si_function b_Z_isLt
+    | "map.hasKey" => si_predicate b_map_hasKey 2 None
+    | "map.lookup" => si_function b_map_lookup
+    | "map.size" => si_function b_map_size
+    | "map.empty" => si_function b_map_empty
+    | "map.update" => si_function b_map_update
+    | _ => si_none
+    end.
+
 End sec2.
-
-
-Module Notations.
-    
-    Notation "'isZ' t" :=
-        ((e_fun
-            b_isZ
-            [(t)]
-        ))
-        (at level 90)
-    .
-
-    Notation "'isString' t" :=
-        ((e_fun
-            b_isString
-            [(t)]
-        ))
-        (at level 90)
-    .
-
-    Notation "'isList' t" :=
-        ((e_fun
-            b_isList
-            [(t)]
-        ))
-        (at level 90)
-    .
-
-    Notation "'isMap' t" :=
-        ((e_fun
-            b_isMap
-            [(t)]
-        ))
-        (at level 90)
-    .
-
-    Notation "'(' x '+Z' y ')'" :=
-        ((e_fun b_Z_plus [(x); (y)]))
-    .
-
-    Notation "'(' x '-Z' y ')'" :=
-        ((e_fun b_Z_minus [(x); (y)]))
-    .
-
-    Notation "'(' x '*Z' y ')'" :=
-        ((e_fun b_Z_times [(x); (y)]))
-    .
-
-    Notation "'(' x '/Z' y ')'" :=
-        ((e_fun b_Z_div [(x); (y)]))
-    .
-
-    Notation "'(' x '<Z' y ')'" :=
-        ((e_fun b_Z_isLt [(x); (y)]))
-    .
-
-    Notation "'(' x '>Z' y ')'" :=
-        ((e_fun b_Z_isLt [(x); (y)]))
-    .
-
-    Notation "'(' x '==Term' y ')'" :=
-        ((e_fun b_term_eq [(x); (y)]))
-    .
-
-    Notation "'(' x '==Z' y ')'" :=
-        ((e_fun b_Z_eq [(x); (y)]))
-    .
-
-    Notation "<opaque map>" := (bv_pmap (PNodes _)) (only printing).
-
-End Notations.
-
+(* 
 Definition builtins_binding : BuiltinsBinding := {|
     bb_function_names := [
         (* Sort predicates *)
@@ -2430,243 +2451,47 @@ Definition builtins_binding : BuiltinsBinding := {|
         ("map.empty", "b_map_empty");
         ("map.update", "b_map_update")
     ];
-|}.
-
-Definition inject_err
-    {symbol : Type}
-    :
-(@BuiltinValue0 symbol)
-:=
-    bv_error
-.
-
-Definition inject_Z
-    {symbol : Type}
-    (Fret :  option (@BuiltinValue0 symbol) -> (@BuiltinValue0 symbol))
-    (z : Z)
-    :
-    (@BuiltinValue0 symbol) :=
-    Fret (Some (bv_Z z))
-.
-
-Definition inject_bool
-    {symbol : Type}
-    (Fret :  option (@BuiltinValue0 symbol) -> (@BuiltinValue0 symbol))
-    (b : bool)
-    :
-    (@BuiltinValue0 symbol) :=
-    Fret (Some (bv_bool b))
-.
-
-Definition inject_string
-    {symbol : Type}
-    (Fret : option (@BuiltinValue0 symbol) -> (@BuiltinValue0 symbol))
-    (s : string)
-    :
-    (@BuiltinValue0 symbol) :=
-    Fret (Some (bv_str s))
-.
-
+|}. *)
+(* 
 Definition eject
     {symbol : Type}
     (v : @BuiltinValue0 symbol)
     :
-    option (bool+(Z+(string+unit)))%type
+    option (bool+(Z+(string)))%type
     :=
     match v with
     | bv_bool b => Some (inl b)
     | bv_Z z => Some (inr(inl z))
-    | bv_str s => Some (inr(inr (inl s)))
-    | bv_error => Some (inr(inr (inr ())))
+    | bv_str s => Some (inr(inr (s)))
     | _ => None
     end 
+. *)
+
+
+(* Print bv_list. *)
+(* 
+Section sb.
+    Context
+        {symbol : Type}
+        (show_symbol : symbol -> string)
+    .
+
+    (* Doing recursion of BuiltinValue0 is really hard. I gave up, as we need to deprecate klike anyway. *)
+    Definition show_builtin
+        (v : @BuiltinValue symbol)
+        : string
+    :=
+        match v with
+        | bv_bool true => "true"
+        | bv_bool false => "false"
+        | bv_Z z => pretty_Z z
+        | bv_sym s => (show_symbol s) +:+ "@sym"
+        | bv_str s => (s) +:+ "@str"
+        | bv_list l =>
+            "<unsupported (list of stuff)>"
+        | bv_pmap p =>
+            "<unsupported (map of stuff)>"
+        end
 .
 
-Section negations.
-    Context
-        (symbol : Type)
-        (variable : Type)
-        (symbols : Symbols symbol)
-        (variables : MVariables variable)
-        (my_program_info : @ProgramInfo symbol symbols MyUnit mysignature (@β symbol symbols))
-        (nondet_gen : nat -> MyUnit)
-    .
-
-    (* #[local] *)
-    Definition Σ := (mkStaticModel
-        symbol
-        variable
-        symbols
-        MyUnit
-        mysignature
-        (@β symbol symbols)
-        variables
-        my_program_info
-        nondet_gen
-    ).
-
-    Ltac2 case_on_length () :=
-        repeat(
-            simpl in *;
-            match! goal with
-            | [h: ((length ?args) = (S _)) |- _] =>
-                destruct $args; simpl in $h; try ltac1:(lia)
-            | [h: ((length ?args) = O) |- _] =>
-                destruct $args; simpl in $h; try ltac1:(lia)
-            | [h: ((S _) = (S _)) |- _] =>
-                apply Nat.succ_inj in $h
-            end
-        )
-    .
-
-    Ltac2 simplify_negable () :=
-        case_on_length ();
-        unfold liftUnaryP,liftNularyP,liftBinaryP;
-        ltac1:(repeat (case_match; simpl in *; simplify_option_eq; try reflexivity));
-        repeat (match! goal with
-        | [ h: (Expression2_evaluate _ _ _ = None) |- _ ] =>
-            apply (@Expression2_evaluate_None_inv Σ) in $h
-        end);
-        unfold vars_of in *; simpl in *
-    .
-
-    Ltac2 solve_negable () := simplify_negable (); ltac1:(set_solver) .
-
-    #[export]
-    Program Instance Negable_isZ : @NegablePredicateSymbol Σ b_isZ 1
-        := {|
-            nps_negate := fun args => sc_atom b_isNotZ args;
-        |}
-    .
-    Next Obligation. intros. solve_negable (). Qed. Fail Next Obligation.
-
-    #[export]
-    Program Instance Negable_isNotZ : @NegablePredicateSymbol Σ b_isNotZ 1
-        := {|
-            nps_negate := fun args => sc_atom b_isZ args;
-        |}
-    .
-    Next Obligation.
-        intros. simplify_negable ().
-        {
-            rewrite negb_involutive. reflexivity.
-        }
-        {
-            ltac1:(set_solver).
-        }
-    Qed.
-    Fail Next Obligation.
-
-
-    #[export]
-    Program Instance Negable_isString : @NegablePredicateSymbol Σ b_isString 1
-        := {|
-            nps_negate := fun args => sc_atom b_isNotString args;
-        |}
-    .
-    Next Obligation. intros. solve_negable (). Qed. Fail Next Obligation.
-
-    #[export]
-    Program Instance Negable_isNotString : @NegablePredicateSymbol Σ b_isNotString 1
-        := {|
-            nps_negate := fun args => sc_atom b_isString args;
-        |}
-    .
-    Next Obligation.
-        intros. simplify_negable ().
-        {
-            rewrite negb_involutive. reflexivity.
-        }
-        {
-            ltac1:(set_solver).
-        }
-    Qed.
-    Fail Next Obligation.
-
-    #[export]
-    Program Instance Negable_isBool : @NegablePredicateSymbol Σ b_isBool 1
-        := {|
-            nps_negate := fun args => sc_atom b_isNotBool args;
-        |}
-    .
-    Next Obligation. intros. solve_negable (). Qed. Fail Next Obligation.
-
-    #[export]
-    Program Instance Negable_isNotBool : @NegablePredicateSymbol Σ b_isNotBool 1
-        := {|
-            nps_negate := fun args => sc_atom b_isBool args;
-        |}
-    .
-    Next Obligation.
-        intros. simplify_negable ().
-        {
-            rewrite negb_involutive. reflexivity.
-        }
-        {
-            ltac1:(set_solver).
-        }
-    Qed.
-    Fail Next Obligation.
-
-    #[export]
-    Program Instance Negable_b_bool_is_true : @NegablePredicateSymbol Σ b_bool_is_true 1
-    := {|
-        nps_negate := fun args => sc_or (sc_atom b_bool_is_false args) (sc_atom b_isNotBool args);
-    |}.
-    Next Obligation.
-        intros. simplify_negable ().
-        {
-            rewrite orb_false_r.
-            destruct b; simpl; reflexivity.
-        }
-        {
-            unfold vars_of in *; simpl in *.
-            ltac1:(set_solver).
-        }
-    Qed.
-    Fail Next Obligation.
-
-    #[export]
-    Program Instance Negable_b_bool_is_false : @NegablePredicateSymbol Σ b_bool_is_false 1
-    := {|
-        nps_negate := fun args => sc_or (sc_atom b_bool_is_true args) (sc_atom b_isNotBool args);
-    |}.
-    Next Obligation.
-        intros. simplify_negable ().
-        {
-            rewrite orb_false_r.
-            destruct b; simpl; reflexivity.
-        }
-        {
-            unfold vars_of in *; simpl in *.
-            ltac1:(set_solver).
-        }
-    Qed.
-    Fail Next Obligation.
-
-  
-    #[export]
-    Program Instance Negable_have_same_symbol_symbol : @NegablePredicateSymbol Σ b_have_same_symbol 2
-    := {|
-        nps_negate := fun args => sc_or (sc_or (sc_atom b_have_different_symbols args) (sc_atom b_isBuiltin (slice 0 1 args))) (sc_atom b_isBuiltin (slice 1 2 args)) ;
-    |}.
-    Next Obligation.
-        intros. simpl.
-        unfold slice.
-        simplify_negable (); unfold vars_of in *; simpl in *; ltac1:(set_solver).
-    Qed.
-    Fail Next Obligation.
-
-    #[export]
-    Program Instance Negable_not_have_same_symbol_symbol : @NegablePredicateSymbol Σ b_have_different_symbols 2
-    := {|
-        nps_negate := fun args => sc_or (sc_or (sc_atom b_have_same_symbol args) (sc_atom b_isBuiltin (slice 0 1 args))) (sc_atom b_isBuiltin (slice 1 2 args)) ;
-    |}.
-    Next Obligation.
-        intros. simpl.
-        unfold slice.
-        simplify_negable (); unfold vars_of in *; simpl in *; ltac1:(set_solver).
-    Qed.
-    Fail Next Obligation.
-
-End negations.
+End sb. *)
