coq-minuska/theories/builtin/int_signature.v
@@ -65,8 +65,24 @@ Next Obligation.
 Qed.
 Fail Next Obligation.
 
-Definition int_signature : Signature := {|
+Program Definition int_signature : Signature := {|
     builtin_function_symbol := IntFunSymbol ;
     builtin_predicate_symbol := IntPredSymbol ;
+    bps_ar := fun p =>
+        match p with
+        | int_is => 1
+        end ;
+    bps_neg := fun p =>
+        match p with
+        | int_is => None
+        end ;
+    bps_neg_ar := _;
+    bps_neg__sym := _;
 |}.
-
+Next Obligation.
+    destruct p,p'; simpl in *; ltac1:(lia).
+Qed.
+Next Obligation.
+    destruct p,p'; simpl in *; ltac1:(simplify_eq/=).
+Qed.
+Fail Next Obligation.
