coq-minuska/theories/default_everything.v
@@ -17,11 +17,26 @@ Require Export
   Coq.extraction.ExtrOcamlBasic(*
   Coq.extraction.ExtrOcamlChar
   Coq.extraction.ExtrOcamlString*)
+  Coq.extraction.ExtrOcamlNativeString
   Coq.extraction.ExtrOcamlZBigInt
   Coq.extraction.ExtrOcamlNatBigInt
 .
 
-(* Set Extraction KeepSingleton. *)
+(* Adapted from [Coq.extraction.ExtrOcamlNativeString], using [Stdlib.String] instead of [String]*)
+Extract Inductive string => "string"
+[
+"
+  """"
+"
+"
+  (fun (c, s) -> Stdlib.String.make 1 c ^ s)
+"
+]
+"
+ (fun f0 f1 s ->
+    let l = Stdlib.String.length s in
+    if l = 0 then f0 () else f1 (Stdlib.String.get s 0) (Stdlib.String.sub s 1 (l-1)))
+".
 
 From Coq Require Import String Bool Arith ZArith List.
 
@@ -54,15 +69,15 @@ Definition gt_over {mysignature : Signature} {β : Model mysignature MyUnit} (b 
 Definition gt_term {mysignature : Signature} {β : Model mysignature MyUnit} (s : string) (l : list GT) : GT := @t_term string builtin_value s l.
 
 Definition basic_rule
-    {mysignature : Signature}
-    {β : Model mysignature MyUnit}
-    (program_info : ProgramInfo)
+    (* {mysignature : Signature} *)
+    (* {β : Model mysignature MyUnit} *)
+    (* (program_info : ProgramInfo) *)
     (name : string)
-    (l : TermOver BuiltinOrVar)
-    (r : TermOver Expression2)
-    (cond : SideCondition) : Declaration
+    (l : @TermOver' string StringBuiltinOrVar)
+    (r : @TermOver' string StringExpression)
+    (cond : StringSideCondition) : Declaration Act
 :=
-    (decl_rule (@mkRuleDeclaration (DSM program_info) Act name (@mkRewritingRule2 (DSM program_info) Act l r cond default_act)))
+    (decl_rule _ (@mkRuleDeclaration Act name (@mkStringRewritingRule Act l r cond default_act)))
 .
 
 
@@ -77,19 +92,59 @@ Definition BoV_to_Expr2
     end
 .
 
-Definition framed_rule
-    {mysignature : Signature}
-    {β : Model mysignature MyUnit}
-    (program_info : ProgramInfo)
-    (frame : (variable*(TermOver BuiltinOrVar)))
-    (name : string)
-    (l : TermOver BuiltinOrVar)
-    (r : TermOver Expression2)
-    (cond : SideCondition) : Declaration
+Fixpoint sTermOverBoV_subst_gen
+    {B : Type}
+    (lift_builtin : BuiltinRepr -> B)
+    (lift_variable : string -> B)
+    (t : @TermOver' string StringBuiltinOrVar)
+    (x : string)
+    (t' : @TermOver' string B)
+    : @TermOver' string B
 :=
-    (decl_rule (@mkRuleDeclaration (DSM program_info) Act name (@mkRewritingRule2 (DSM program_info) Act
-        (TermOverBoV_subst frame.2 frame.1 l)
-        (TermOverBoV_subst_expr2 frame.2 frame.1 r)
+match t with
+| t_over (sbov_builtin b) => t_over (lift_builtin b)
+| t_over (sbov_var y) =>
+    match (decide (x = y)) with
+    | left _ => t'
+    | right _ => t_over (lift_variable y)
+    end
+| t_term s l => t_term s (map (fun t'' => sTermOverBoV_subst_gen lift_builtin lift_variable t'' x t') l)
+end.
+
+Definition sTermOverBoV_subst_expr2
+    (t : @TermOver' string StringBuiltinOrVar)
+    (x : string)
+    (t' : @TermOver' string StringExpression)
+    : @TermOver' string StringExpression
+:=
+    sTermOverBoV_subst_gen (fun b => se_ground (t_over b)) (fun x => se_variable x) t x t'
+.
+
+Fixpoint sTermOverBoV_subst
+    (t : @TermOver' string StringBuiltinOrVar)
+    (x : string)
+    (t' : @TermOver' string StringBuiltinOrVar)
+:=
+match t with
+| t_over (sbov_builtin b) => t_over (sbov_builtin b)
+| t_over (sbov_var y) =>
+    match (decide (x = y)) with
+    | left _ => t'
+    | right _ => t_over (sbov_var y)
+    end
+| t_term s l => t_term s (map (fun t'' => sTermOverBoV_subst t'' x t') l)
+end.
+
+Definition framed_rule
+    (frame : (string*(@TermOver' string StringBuiltinOrVar)))
+    (name : string)
+    (l : @TermOver' string StringBuiltinOrVar)
+    (r : @TermOver' string StringExpression)
+    (cond : StringSideCondition) : Declaration Act
+:=
+    (decl_rule _ (@mkRuleDeclaration Act name (@mkStringRewritingRule Act
+        (sTermOverBoV_subst frame.2 frame.1 l)
+        (sTermOverBoV_subst_expr2 frame.2 frame.1 r)
         cond default_act)))
 .
 
