flake.nix
@@ -76,7 +76,10 @@
             cp dune-project $out/
             cp bin/* $out/bin
             cp lib/* $out/lib
-            cp ${coqMinuska}/share/coq-minuska/Dsm.ml ${coqMinuska}/share/coq-minuska/Dsm.mli $out/lib/
+            cp ${coqMinuska}/share/coq-minuska/Dsm.mli $out/lib/
+            printf "open Stdlib\n" >> $out/lib/Dsm.ml
+            cat ${coqMinuska}/share/coq-minuska/Dsm.ml >> $out/lib/Dsm.ml
+
             ls -R $out
           '';
 
@@ -207,6 +210,8 @@
             self.outputs.packages.${system}.minuska
             pkgs.dune_3
             pkgs.time
+            pkgs.coqPackages_8_19.coqide # for user builtins
+            pkgs.coqPackages_8_19.coq
           ] ++ example_languages_parser_deps;
           buildInputs = [
             self.outputs.packages.${system}.coq-minuska
