languages/decrement-builtin/def.m
@@ -3,10 +3,10 @@
 @context(HOLE): cfg [ HOLE ];
 @strictness: [];
 
-@rule [init]: builtin.init[] => cfg[program.ast()] where @true ;
+@rule [init]: builtin.init[] => cfg[@query:program.ast()] where @true ;
 
 @rule [decrement]:
-	cfg[X] => cfg[z.minus(X, [(@builtin-int 1)])] where @true
+	cfg[X] => cfg[z.minus(X, [(@builtin:int("1"))])] where @true
     ;
 
 
